Adding threaded counter example.

progs/threaded_counter.c
@@ -1,28 +1,60 @@
 #include <pthread.h>
 
-void *incr();
 
-pthread_mutex_t mutex1 = PTHREAD_MUTEX_INITIALIZER;
-int  counter = 0;
+/* the lock*/
+pthread_mutex_t ctr_mutex = PTHREAD_MUTEX_INITIALIZER;
+
+/* The counter part */
+
+int zero = 0;
+int *ctr = &zero;
+
+void reset() {
+  int* ctr0 = ctr;
+  *ctr0 = 0;
+}
+
+void *incr() {
+   pthread_mutex_lock( &ctr_mutex );
+   int* ctr0 = ctr;
+   int t = *ctr0;
+   *ctr0 = t +2;
+   /* printf("Counter is: %d \n", *ctr); */
+   pthread_mutex_unlock( &ctr_mutex );
+}
+
+int read() {
+  int* ctr0 = ctr;
+  int t = *ctr0;
+  return t;
+}
+
+/* The threaded part */
+void *thread_incr(void *arg) {
+   pthread_mutex_t *thread_mutex_ptr = (pthread_mutex_t *)arg;
+   incr();
+   pthread_mutex_unlock( thread_mutex_ptr );
+}
 
 int  main(void)
 {
-   int rc1, rc2;
+  
+   /* ctr = 0 */
+   reset();
+   int rc1;
+   pthread_mutex_t thread_mutex = PTHREAD_MUTEX_INITIALIZER;
+   pthread_mutex_lock( &thread_mutex );
+   pthread_t thread1;
+   /* Spawn */
+   rc1=pthread_create( &thread1, NULL, thread_incr, &thread_mutex);
    
-   pthread_t thread1, thread2;
+   /*Local incr */
+   incr();
 
-   rc1=pthread_create( &thread1, NULL, &incr, NULL);
-
-   rc2=pthread_create( &thread2, NULL, &incr, NULL);
-   pthread_join( thread1, NULL);
-   pthread_join( thread2, NULL); 
-
-   return 1;
-}
-
-void *incr()
-{
-   pthread_mutex_lock( &mutex1 );
-   counter++;
-   pthread_mutex_unlock( &mutex1 );
+   /*JOIN */
+   pthread_mutex_lock( &thread_mutex );
+   /* printf("I'm done with a final counter of: %d\n", *ctr); */
+    
+   int t = read();
+   return t;
 }
