progs/verif_threaded_counter.v
@@ -3,11 +3,29 @@ Load threaded_counter.
 
 Local Open Scope logic.
 
-Definition t_struct_mutex1 := Tstruct _mutex1 noattr.
-Definition t_struct_counter := Tstruct _counter noattr.
 
-Definition incr_spec :=
- DECLARE _main
+Instance CompSpecs : compspecs.
+Proof. make_compspecs prog. Defined.  
+
+Definition t_struct_mutex1 := Tstruct _ctr_mutex noattr.
+
+Definition t_struct_zero := Tstruct _zero noattr.
+Definition t_struct_ctr := Tstruct _ctr noattr.
+
+Definition reset_spec :=
+ DECLARE _reset
+  WITH z : int, addof_ctr: val, ctr: val
+  PRE  [] 
+        PROP ()
+        LOCAL(gvar _ctr addof_ctr)
+        SEP(`(data_at Ews tint (repinj tint z) ctr);`(data_at Ews (tptr tint) ctr addof_ctr))
+  POST [tvoid]
+        PROP()
+        LOCAL()
+        SEP(`(data_at Ews tint (repinj tint Int.zero) ctr);`(data_at Ews (tptr tint) ctr addof_ctr)).
+
+Definition read_spec :=
+ DECLARE _read
   WITH z : int, addof_ctr: val, ctr: val
   PRE  [] 
         PROP ()
@@ -15,5 +33,68 @@ Definition incr_spec :=
         SEP(`(data_at Ews tint (repinj tint z) ctr);`(data_at Ews (tptr tint) ctr addof_ctr))
   POST [tint]
         PROP()
+        LOCAL( temp ret_temp (Vint z))
+        SEP(`(data_at Ews tint (repinj tint z) ctr);`(data_at Ews (tptr tint) ctr addof_ctr)).
+
+Definition incr_spec :=
+ DECLARE _incr
+  WITH z : int, addof_ctr: val, ctr: val
+  PRE  [] 
+        PROP ()
+        LOCAL()
+        SEP()
+  POST [tvoid]
+        PROP()
+        LOCAL()
+        SEP().
+
+Definition main_spec :=
+ DECLARE _main
+  WITH z0 : int, z1 : int, addof_ctr: val, ctr: val
+  PRE  [] 
+        PROP ()
+        LOCAL(gvar _ctr addof_ctr)
+        SEP(`(data_at Ews tint (repinj tint z0) ctr);`(data_at Ews (tptr tint) ctr addof_ctr))
+  POST [tint]
+        PROP()
         LOCAL( temp ret_temp (Vint (Int.repr 2)))
-        SEP(`(data_at Ews tint (repinj tint (Int.add (Int.add Int.zero Int.one) Int.one)) ctr);`(data_at Ews (tptr tint) ctr addof_ctr)).
+        SEP(`(data_at Ews tint (repinj tint z1) ctr);`(data_at Ews (tptr tint) ctr addof_ctr)).
+
+Definition Vprog : varspecs := (_ctr_mutex, )::(_ctr, tptr tint)::(_zero,tint)::nil.
+
+Definition Gprog : funspecs := 
+  reset_spec::incr_spec::read_spec::main_spec::nil.
+
+Definition main_spec :=
+ DECLARE _main
+  WITH z : int, addof_ctr: val, ctr: val
+  PRE  [] 
+        PROP ()
+        LOCAL(gvar _counter addof_ctr)
+        SEP(`(data_at Ews tint (repinj tint z) ctr);`(data_at Ews (tptr tint) ctr addof_ctr))
+  POST [tint]
+        PROP()
+        LOCAL( temp ret_temp (Vint (Int.one)))
+        SEP(`(data_at Ews tint (repinj tint z) ctr);`(data_at Ews (tptr tint) ctr addof_ctr)).
+
+Definition Vprog : varspecs := (_counter, tptr tint)::nil.
+
+Definition Gprog : funspecs := 
+  main_spec::nil.
+
+Lemma body_main:  semax_body Vprog Gprog f_main main_spec.
+Proof.
+ start_function.
+ name ctr_ _counter.
+ forward.
+ eapply semax_seq.
+ eapply semax_post.
+ 
+ forward.
+ 
+ forward_call' (z, addof_ctr, ctr).
+ forward_call' (Int.zero, addof_ctr, ctr).
+ forward_call' ((Int.add Int.zero Int.one), addof_ctr, ctr).
+ forward_call' ((Int.add (Int.add Int.zero Int.one) Int.one), addof_ctr, ctr) r0.
+ forward.
+Qed.
